coq/theories/utils/Words4Naive.v
@@ -14,8 +14,9 @@ Definition ok width: 0 < width -> word.ok (word width) :=
   gen_ok width (default_special_case_handlers width).
 
 Notation word4 := (word 4).
+
 #[global] Instance word4_ok : word.ok word4 := ok 4 eq_refl.
-Add Ring wring8 : (Properties.word.ring_theory (word := word4))
+Add Ring wring4 : (Properties.word.ring_theory (word := word4))
       (preprocess [autorewrite with rew_word_morphism],
        morphism (Properties.word.ring_morph (word := word4)),
        constants [Properties.word_cst]).
